Yet another refactor. triples got own file

src/Rdf.v
@@ -2,125 +2,17 @@ From Coq Require Import Lists.ListSet.
 From Coq Require Import Init.Nat.
 From Coq Require Import Strings.String.
 From Coq Require Import Bool.Bool.
-From Coq Require Import Arith.EqNat.
 From RDF Require Import Term.
 From RDF Require Import Maps.
+From RDF Require Import Triple.
 
-Inductive trpl : Type :=
-  | triple (s p o : term).
-
-
-Theorem eq_nat_eq_lit : forall (n1 n2:nat) , (n1 = n2) <-> (Lit n1) = (Lit n2).
-Proof. split; intros H.
-  - rewrite H. reflexivity.
-  - injection H as H2. apply H2.
-Qed.
-
-Theorem eq_string_eq_iri : forall (s1 s2:string) , (s1 = s2) <-> (Iri s1) = (Iri s2).
-Proof. split; intros H.
-  - rewrite H. reflexivity.
-  - injection H as H2. apply H2.
-Qed.
-
-Theorem eq_string_eq_bnode : forall (s1 s2:string) , (s1 = s2) <-> (Bnode s1) = (Bnode s2).
-Proof. split; intros H.
-  - rewrite H. reflexivity.
-  - injection H as H2. apply H2.
-Qed.
-
-Theorem eqb_node_refl : forall (nod1 : term),
-  true = eqb_node nod1 nod1.
-Proof. destruct nod1 as []; simpl.
-  - symmetry. apply eqb_refl.
-  - apply beq_nat_refl.
-  - symmetry. apply eqb_refl.
-Qed.
-
-Theorem eqb_eq_node : forall (nod1 nod2 : term),
-  eqb_node nod1 nod2 = true <-> nod1 = nod2.
-Proof. split; intros H.
-  - destruct nod1,nod2 as [] ; 
-    try reflexivity ;
-    try discriminate; simpl in H.
-    + apply eqb_eq in H. rewrite H. apply eq_string_eq_iri. reflexivity.
-    + apply beq_nat_true in H. rewrite H. apply eq_nat_eq_lit. reflexivity.
-    + apply eqb_eq in H. apply eq_string_eq_bnode. apply H.
-  - rewrite H. symmetry. apply eqb_node_refl.
-Qed.
-   
-Theorem eqb_neq_node : forall (nod1 nod2 : term),
-  eqb_node nod1 nod2 = false <-> nod1 <> nod2.
-Proof. split.
-  - intros H contra. rewrite contra in H. rewrite <- eqb_node_refl in H. discriminate H.
-  - intros H. unfold not in H. rewrite <- eqb_eq_node in H. destruct (eqb_node nod1 nod2) as [].
-    + exfalso. apply H. reflexivity.
-    + reflexivity.
-Qed.
-
-(* alias for triple of terms type *)
-(* Definition triple := (node * term * term)%type.  *)
-
-(*
-   Inductive rdf : Type :=
-  | graph (triples : list triple).
- *)
 
 (* Not sure if its a good idea to have a set, 
  may be we want some order on the triples *)
 Definition graph := set trpl.
 
-Definition app_μ_to_triple (μ : term -> term) (t : trpl) : trpl:=
-  (match t with
-   | (triple n1 n2 n3) => triple (μ n1) n2 (μ n3)
-   end).
-
-Theorem eq_dec_node : forall (n m: term),
-  {n = m} + {n <> m}.
-Proof. decide equality.
-  + apply string_dec.
-  + decide equality.
-  + apply string_dec.
-Qed.
-
-
-Definition eqb_triple (t1 t2:trpl) : bool :=
-  (match t1,t2 with
-   | (triple s p o),(triple s2 p2 o2) => (eqb_node s s2) && (eqb_node p p2) && (eqb_node o o2)
-   end).
-
-Theorem eqb_eq_triple: forall (t1 t2 : trpl),
-  eqb_triple t1 t2 = true <-> t1 = t2.
-Proof. intros. split; intros H.
-  - destruct t1,t2 as [s2 p2 o2]; f_equal;
-    simpl in H; apply andb_true_iff in H; destruct H as [H0 H2]; apply andb_true_iff in H0; destruct H0 as [H H1]; apply eqb_eq_node. 
-    + apply H.
-    + apply H1.
-    + apply H2.
-  - destruct t1,t2 as [s2 p2 o2]. injection H as H1 H2 H3. simpl. rewrite H1. rewrite H2. rewrite H3.
-    rewrite <- (eqb_node_refl s2). rewrite <- (eqb_node_refl p2). rewrite <- (eqb_node_refl o2). reflexivity.
-Qed.
-
-Theorem eqb_triple_refl : forall (t1: trpl),
-  eqb_triple t1 t1 = true.
-Proof. intros. destruct t1. simpl. rewrite <- (eqb_node_refl s). rewrite <- (eqb_node_refl p). rewrite <- (eqb_node_refl o). reflexivity.
-Qed.
-
-Theorem eqb_neq_triple : forall (t1 t2: trpl),
-  eqb_triple t1 t2 = false <-> t1 <> t2.
-Proof. intros. split.
-  - intros H contra. rewrite contra in H. rewrite eqb_triple_refl in H. discriminate H.
-  - intros H. unfold not in H. rewrite <- eqb_eq_triple in H. destruct (eqb_triple t1 t2).
-    + exfalso. apply H. reflexivity.
-    + reflexivity.
-Qed.
-
-Theorem eq_dec_triple : forall (t1 t2: trpl),
-  {t1 = t2} + {t1 <> t2}.
-Proof. decide equality; try decide equality; try apply string_dec; decide equality. Qed.
-
 Definition image (g : graph) (μ : term -> term) : graph :=
   set_map eq_dec_triple (fun t => app_μ_to_triple μ t) g.
-
 
 Definition eqb_graph (g g': graph) : bool :=
   (match (set_diff eq_dec_triple g g') with
@@ -129,23 +21,23 @@ Definition eqb_graph (g g': graph) : bool :=
    end).
 
 Inductive world : Type :=
-  | res (I L B : set term).
+  | res (I L B : set term) (P : set_inter eq_dec_term I (set_inter eq_dec_term L B) = empty_set term).
 
 Definition proj_I (w : world) : set term :=
   match w with
-  | res i _ _ => i
+  | res i _ _ _ => i
   end.
 Definition proj_L (w : world) : set term :=
   match w with
-  | res _ l _ => l
+  | res _ l _ _ => l
   end.
 
 Definition proj_B (w : world) : set term :=
   match w with
-  | res _ _ b => b
+  | res _ _ b _ => b
   end.
 Definition proj_IL (w : world) : set term:=
-  set_union eq_dec_node (proj_I w) (proj_L w).
+  set_union eq_dec_term (proj_I w) (proj_L w).
 
 Definition isomorphism (w : world) (g g': graph) :=
   exists μ : term -> term,
