src/Term.v
@@ -1,5 +1,6 @@
 From Coq Require Import Init.Nat.
 From Coq Require Import Strings.String.
+From Coq Require Import Arith.EqNat.
 
 Definition eqb_string (x y : string) : bool :=
   if string_dec x y then true else false.
@@ -28,10 +29,66 @@ Definition is_bnode (n : term) : bool :=
    | _ => false
    end).
 
-Definition eqb_node (n1 n2 : term) : bool :=
+Definition eqb_term (n1 n2 : term) : bool :=
   (match n1, n2 with
    | (Iri id), (Iri id2) => eqb id id2
    | (Lit l),(Lit l2) => l =? l2
    | (Bnode b),(Bnode b2) => eqb b b2
    | _,_ => false
    end).
+
+Theorem eq_nat_eq_lit : forall (n1 n2:nat) , (n1 = n2) <-> (Lit n1) = (Lit n2).
+Proof. split; intros H.
+  - rewrite H. reflexivity.
+  - injection H as H2. apply H2.
+Qed.
+
+Theorem eq_string_eq_iri : forall (s1 s2:string) , (s1 = s2) <-> (Iri s1) = (Iri s2).
+Proof. split; intros H.
+  - rewrite H. reflexivity.
+  - injection H as H2. apply H2.
+Qed.
+
+Theorem eq_string_eq_bnode : forall (s1 s2:string) , (s1 = s2) <-> (Bnode s1) = (Bnode s2).
+Proof. split; intros H.
+  - rewrite H. reflexivity.
+  - injection H as H2. apply H2.
+Qed.
+
+Theorem eq_dec_term : forall (t1 t2: term),
+  {t1 = t2} + {t1 <> t2}.
+Proof. decide equality.
+  + apply string_dec.
+  + decide equality.
+  + apply string_dec.
+Qed.
+
+Theorem eqb_term_refl : forall (t1 : term),
+  eqb_term t1 t1 = true.
+Proof. destruct t1 as []; simpl.
+  - apply eqb_refl.
+  - symmetry. apply beq_nat_refl.
+  - apply eqb_refl.
+Qed.
+
+Theorem eqb_eq_term : forall (t1 t2 : term),
+  eqb_term t1 t2 = true <-> t1 = t2.
+Proof. split; intros H.
+  - destruct t1,t2 as [] ; 
+    try reflexivity ;
+    try discriminate; simpl in H.
+    + apply eqb_eq in H. rewrite H. apply eq_string_eq_iri. reflexivity.
+    + apply beq_nat_true in H. rewrite H. apply eq_nat_eq_lit. reflexivity.
+    + apply eqb_eq in H. apply eq_string_eq_bnode. apply H.
+  - rewrite H. apply eqb_term_refl.
+Qed.
+   
+Theorem eqb_neq_term : forall (t1 t2 : term),
+  eqb_term t1 t2 = false <-> t1 <> t2.
+Proof. split.
+  - intros H contra. rewrite contra in H. rewrite eqb_term_refl in H. discriminate H.
+  - intros H. unfold not in H. rewrite <- eqb_eq_term in H. destruct (eqb_term t1 t2) as [].
+    + exfalso. apply H. reflexivity.
+    + reflexivity.
+Qed.
+
