src/Triple.v
@@ -1,0 +1,56 @@
+From RDF Require Import Term.
+From Coq Require Import Lists.ListSet.
+From Coq Require Import Init.Nat.
+From Coq Require Import Strings.String.
+From Coq Require Import Bool.Bool.
+
+Inductive trpl : Type :=
+  | triple (s p o : term).
+
+(* alias for triple of terms type *)
+(* Definition triple := (node * term * term)%type.  *)
+
+(*
+   Inductive rdf : Type :=
+  | graph (triples : list triple).
+ *)
+
+Definition app_μ_to_triple (μ : term -> term) (t : trpl) : trpl:=
+  (match t with
+   | (triple n1 n2 n3) => triple (μ n1) n2 (μ n3)
+   end).
+
+Definition eqb_triple (t1 t2:trpl) : bool :=
+  (match t1,t2 with
+   | (triple s p o),(triple s2 p2 o2) => (eqb_term s s2) && (eqb_term p p2) && (eqb_term o o2)
+   end).
+
+Theorem eqb_eq_triple: forall (t1 t2 : trpl),
+  eqb_triple t1 t2 = true <-> t1 = t2.
+Proof. intros. split; intros H.
+  - destruct t1,t2 as [s2 p2 o2]; f_equal;
+    simpl in H; apply andb_true_iff in H; destruct H as [H0 H2]; apply andb_true_iff in H0; destruct H0 as [H H1]; apply eqb_eq_term. 
+    + apply H.
+    + apply H1.
+    + apply H2.
+  - destruct t1,t2 as [s2 p2 o2]. injection H as H1 H2 H3. simpl. rewrite H1. rewrite H2. rewrite H3.
+    rewrite (eqb_term_refl s2). rewrite (eqb_term_refl p2). rewrite (eqb_term_refl o2). reflexivity.
+Qed.
+
+Theorem eqb_triple_refl : forall (t1: trpl),
+  eqb_triple t1 t1 = true.
+Proof. intros. destruct t1. simpl. rewrite (eqb_term_refl s). rewrite (eqb_term_refl p). rewrite (eqb_term_refl o). reflexivity.
+Qed.
+
+Theorem eqb_neq_triple : forall (t1 t2: trpl),
+  eqb_triple t1 t2 = false <-> t1 <> t2.
+Proof. intros. split.
+  - intros H contra. rewrite contra in H. rewrite eqb_triple_refl in H. discriminate H.
+  - intros H. unfold not in H. rewrite <- eqb_eq_triple in H. destruct (eqb_triple t1 t2).
+    + exfalso. apply H. reflexivity.
+    + reflexivity.
+Qed.
+
+Theorem eq_dec_triple : forall (t1 t2: trpl),
+  {t1 = t2} + {t1 <> t2}.
+Proof. decide equality; try decide equality; try apply string_dec; decide equality. Qed.
