src/examples/RdfExamples.v
@@ -1,14 +1,15 @@
 From RDF Require Import Term.
+From RDF Require Import Triple.
 From RDF Require Import Rdf. 
 From Coq Require Import Strings.String.
 From Coq Require Import Lists.ListSet.
 
 Check (triple (Bnode "a") (Lit 1) (Iri "foo")): trpl.
 
-Check (set_add eq_dec_node (Iri "x") (set_add eq_dec_node (Lit 5) (empty_set term))).
+Check (set_add eq_dec_term (Iri "x") (set_add eq_dec_term (Lit 5) (empty_set term))).
 
-Example example_in_graph : set_In (Lit 12) (set_add eq_dec_node (Lit 12) (set_add eq_dec_node (Lit 5) (empty_set term))).
-Proof. simpl. destruct (eq_dec_node (Lit 12) (Lit 5)) eqn:E.
+Example example_in_graph : set_In (Lit 12) (set_add eq_dec_term (Lit 12) (set_add eq_dec_term (Lit 5) (empty_set term))).
+Proof. simpl. destruct (eq_dec_term (Lit 12) (Lit 5)) eqn:E.
   - simpl. left. symmetry. apply e.
   - simpl. right. left. reflexivity.
 Qed.
@@ -25,4 +26,3 @@ Proof. reflexivity. Qed.
 Example eqb_graph_test2 : 
   eqb_graph (set_add eq_dec_triple (triple (Lit 5) (Lit 4) (Lit 3)) (empty_set trpl)) (empty_set trpl) = false.
 Proof. reflexivity. Qed.
-
